Adding more specs to libra_account.
This adds more (now ~50%) specifications to our copy of libra account. All specs do verify. It also extends the translator
to correctly deal with conditions on native functions, to handle the ExistsTxnSenderAccount builtin precondition, and to
constraint integers better.

There are a number of issues this unearthed:

- The specs are very repetitive. We definitely need to think about abstractions to make them more readable.
- We definitely also need better ways to analyze boogie traces and models. The models are completely unusable. Would be nice
  to combine the traces and models somehow.
- We currently cannot write `old(global_exists(...))` (restriction of spec AST and parser), but we need this to represent certain conditions.
  There is a TODO in the code.
- The bug about LibraAccount.create_account turned out (after offline sync with Sam) more to be an ambigious documentation of a native
  function. After correcting this it's fixed (and with the spec the native function's doc is now clear ;-)
- There is possibly another bug in `LibraAccount.pay_from_sender(payee, amount)`. Specifically, payee can be txn_sender. This doesn't
  seem right so I "corrected" this bug and added a TODO to further investigate.

Closes: #2239
Approved by: sblackshear

language/move-prover/bytecode-to-boogie/src/translator.rs
@@ -204,10 +204,20 @@ impl<'a> BoogieTranslator<'a> {
                 }
 
                 let type_value = format!("StructType({}, {})", struct_name, field_types);
-                emit_str(&format!(
-                    "function {}_type_value({}): TypeValue {{\n    {}\n}}\n",
-                    struct_name, type_args, type_value
-                ));
+                if struct_name == "LibraAccount_T" {
+                    // Special treatment of well-known resource LibraAccount_T. The type_value
+                    // function is forward-declared in the prelude, here we only add an axiom for
+                    // it.
+                    emit_str(&format!(
+                        "axiom {}_type_value() == {};\n",
+                        struct_name, type_value
+                    ));
+                } else {
+                    emit_str(&format!(
+                        "function {}_type_value({}): TypeValue {{\n    {}\n}}\n",
+                        struct_name, type_args, type_value
+                    ));
+                }
 
                 // Emit other struct specific boilerplate.
                 if !struct_def_view.is_native() {
@@ -303,6 +313,8 @@ impl<'a> ModuleTranslator<'a> {
             if function_def.is_native() {
                 res.push_str(&self.generate_function_sig(idx, true, &None));
                 res.push_str(";");
+                res.push_str(&self.generate_function_spec(idx, &None));
+                res.push_str("\n");
                 continue;
             }
             res.push_str(&self.translate_function(idx));
@@ -904,10 +916,17 @@ impl<'a> ModuleTranslator<'a> {
             }
             rets.push_str(&format!("ret{}", i));
         }
+        let assumptions = "    assume ExistsTxnSenderAccount(m, txn);\n";
         if function_signature.return_types.is_empty() {
-            format!("\n{{\n    call {}({});\n}}\n\n", fun_name, args)
+            format!(
+                "\n{{\n{}    call {}({});\n}}\n\n",
+                assumptions, fun_name, args
+            )
         } else {
-            format!("\n{{\n    call {} := {}({});\n}}\n\n", rets, fun_name, args)
+            format!(
+                "\n{{\n{}    call {} := {}({});\n}}\n\n",
+                assumptions, rets, fun_name, args
+            )
         }
     }
 
@@ -1155,7 +1174,7 @@ pub fn format_type_checking(
     let mut params = name;
     let mut ret = String::new();
     let check = match sig {
-        SignatureToken::U8 | SignatureToken::U64 | SignatureToken::U128 => "is#Integer",
+        SignatureToken::U8 | SignatureToken::U64 | SignatureToken::U128 => "IsValidInteger",
         SignatureToken::Bool => "is#Boolean",
         SignatureToken::Address => "is#Address",
         SignatureToken::ByteArray => "is#ByteArray",
